pseudo commute is just abel_semigroup

Fold.thy
@@ -1,55 +1,46 @@
 theory Fold imports Main begin
 
-fun foldl :: "('b \<Rightarrow> 'a \<Rightarrow> 'b) \<Rightarrow> 'b \<Rightarrow> 'a list \<Rightarrow> 'b" where
+
+fun
+  foldl :: "('b \<Rightarrow> 'a \<Rightarrow> 'b) \<Rightarrow> 'b \<Rightarrow> 'a list \<Rightarrow> 'b"
+where
   foldl_Nil: "foldl f b [] = b" |
   foldl_Cons: "foldl f b (a#as) = foldl f (f b a) as"
 
-lemma foldl_Cons_sym: "foldl f (f b a) as = foldl f b (a#as)"
-  apply(subst foldl_Cons)
-  apply(rule refl)
-  done
 
-lemma foldl_append1[iff]: "foldl f b (as@[a]) = f (foldl f b as) a"
-  apply(induction as arbitrary: b)
-  apply(simp)
-  apply(subst foldl_Cons)
-  apply(subgoal_tac "(aa#as)@[a] = aa#(as@[a])")
-  apply(erule_tac t="(aa#as)@[a]" in ssubst)
-  apply(subst foldl_Cons)
-  apply(auto)
-  done
-
-fun foldr :: "('b \<Rightarrow> 'a \<Rightarrow> 'b) \<Rightarrow> 'b \<Rightarrow> 'a list \<Rightarrow> 'b" where
+fun
+  foldr :: "('b \<Rightarrow> 'a \<Rightarrow> 'b) \<Rightarrow> 'b \<Rightarrow> 'a list \<Rightarrow> 'b"
+where
   foldr_rev: "foldr f b as = foldl f b (rev as)"
 
-lemma foldr_Nil: "foldr f b [] = b"
-  apply(auto)
-  done
 
-lemma foldr_rev_sym: "foldl f b (rev as) = foldr f b as"
-  apply(subst foldr_rev)
+theorem abel_semigroup_flip: "\<lbrakk> abel_semigroup f \<rbrakk> \<Longrightarrow> f (f b a1) a2 = f (f b a2) a1"
+  apply(unfold abel_semigroup_def semigroup_def abel_semigroup_axioms_def)
+  apply(clarify)
+  apply(frule_tac x=b and P="\<lambda>a. \<forall>b c. f (f a b) c = f a (f b c)" in spec)
+  apply(drule_tac x=a1 and P="\<lambda>ba. \<forall>c. f (f b ba) c = f b (f ba c)" in spec)
+  apply(drule_tac x=a2 and P="\<lambda>c. f (f b a1) c = f b (f a1 c)" in spec)
+  apply(erule ssubst)
+  apply(drule_tac x=a1 and P="\<lambda>a. \<forall>b. f a b = f b a" in spec)
+  apply(drule_tac x=a2 and P="\<lambda>b. f a1 b = f b a1" in spec)
+  apply(erule ssubst)
+  apply(drule_tac x=b and P="\<lambda>a. \<forall>b c. f (f a b) c = f a (f b c)" in spec)
+  apply(drule_tac x=a2 and P="\<lambda>ba. \<forall>c. f (f b ba) c = f b (f ba c)" in spec)
+  apply(drule_tac x=a1 in spec)
+  apply(erule subst)
   apply(rule refl)
   done
 
-definition pseudo_commute :: "('b \<Rightarrow> 'a \<Rightarrow> 'b) \<Rightarrow> bool" where
-  "pseudo_commute f \<equiv> (\<forall>b a1 a2. f (f b a1) a2 = f (f b a2) a1)"
 
-theorem pseudo_commute_iff[iff]: "\<lbrakk> pseudo_commute f \<rbrakk> \<Longrightarrow> f (f b a1) a2 = f (f b a2) a1"
-  apply(unfold pseudo_commute_def)
-  apply(drule_tac x=b in spec)
-  apply(drule_tac x=a1 in spec)
-  apply(erule_tac x=a2 in spec)
-  done
-
-lemma foldl_flip_ends: "\<lbrakk> pseudo_commute f \<rbrakk> \<Longrightarrow> foldl f b (xs@[x]) = foldl f b (x#xs)"
+lemma foldl_flip_ends: "\<lbrakk> abel_semigroup f \<rbrakk> \<Longrightarrow> foldl f b (xs@[x]) = foldl f b (x#xs)"
   apply(induction xs arbitrary: b)
   apply(subst append_Nil)
   apply(rule refl)
   apply(subst foldl_Cons)
   apply(subst foldl_Cons)
-  apply(subst pseudo_commute_iff[of "f"])
+  apply(subst abel_semigroup_flip[of "f"])
   apply(assumption)
-  apply(subst foldl_Cons_sym)
+  apply(subst foldl_Cons[symmetric])
   apply(subst append_Cons)
   apply(subst foldl_Cons)
   apply(drule_tac x="f b a" in meta_spec)
@@ -57,54 +48,25 @@ lemma foldl_flip_ends: "\<lbrakk> pseudo_commute f \<rbrakk> \<Longrightarrow> f
   apply(assumption)
   done
 
-lemma foldl_rev: "\<lbrakk> pseudo_commute f \<rbrakk> \<Longrightarrow> foldl f b (rev as) = foldl f b as"
+
+lemma foldl_rev: "\<lbrakk> abel_semigroup f \<rbrakk> \<Longrightarrow> foldl f b (rev as) = foldl f b as"
   apply(induction as arbitrary: b)
-  apply(simp)
+  apply(subst rev.simps(1))
+  apply(rule refl)
   apply(subst foldl_Cons)
-  apply(subgoal_tac "rev (a#as) = (rev as)@[a]")
-  apply(erule ssubst)
+  apply(subst rev.simps(2))
   apply(subst foldl_flip_ends)
   apply(assumption)
   apply(subst foldl_Cons)
   apply(drule_tac x="f b a" in meta_spec)
   apply(assumption)
-  apply(simp)
   done
 
-theorem foldlr_iff: "\<lbrakk> pseudo_commute f \<rbrakk> \<Longrightarrow> foldl f b as = foldr f b as"
+
+theorem foldlr_iff: "\<lbrakk> abel_semigroup f \<rbrakk> \<Longrightarrow> foldl f b as = foldr f b as"
   apply(subst foldr_rev)
   apply(subst foldl_rev)
   apply(assumption)
   apply(rule refl)
   done
-
-definition assoc :: "('a \<Rightarrow> 'a \<Rightarrow> 'a) \<Rightarrow> bool" where
-  "assoc f \<equiv> \<forall>a b. f a b = f b a"
-
-definition commute :: "('a \<Rightarrow> 'a \<Rightarrow> 'a) \<Rightarrow> bool" where
-  "commute f \<equiv> \<forall>a b c. f (f a b) c = f a (f b c)"
-
-theorem pseudo_commuteI[intro]: "\<lbrakk> assoc f; commute f \<rbrakk> \<Longrightarrow> pseudo_commute f"
-  apply(unfold assoc_def)
-  apply(unfold commute_def)
-  apply(unfold pseudo_commute_def)
-  apply(intro allI)
-  apply(frule_tac x="b" and P="\<lambda>a. \<forall>b c. f (f a b) c = f a (f b c)" in spec)
-  apply(drule_tac x="a1" and P="\<lambda>ba. \<forall>c. f (f b ba) c = f b (f ba c)" in spec)
-  apply(drule_tac x="a2" and P="\<lambda>c. f (f b a1) c = f b (f a1 c)" in spec)
-  apply(erule ssubst)
-  apply(drule_tac x="a1" and P="\<lambda>a. \<forall>b. f a b = f b a" in spec)
-  apply(drule_tac x="a2" and P="\<lambda>b. f a1 b = f b a1" in spec)
-  apply(erule ssubst)
-  apply(drule_tac x="b" in spec)
-  apply(drule_tac x="a2" in spec)
-  apply(drule_tac x="a1" in spec)
-  apply(erule subst)
-  apply(rule refl)
-  done
-
-theorem "\<lbrakk> assoc f; commute f \<rbrakk> \<Longrightarrow> foldl f b as = foldr f b as"
-  apply(drule pseudo_commuteI)
-  apply(assumption)
-  apply(erule foldlr_iff)
-  done
+end
